updating up to slicing. Removing dependencies on msl/rmaps

msl/rmaps.v
@@ -5,9 +5,17 @@ Module Type ADR_VAL.
 Parameter address : Type.
 Parameter some_address:address.
 
+Parameter kind: Type.
+Parameter kjoin: Join kind.
+(*Parameter kind_pcm: @PCM kind kjoin.*)
+Parameter kind_ppcm: @PrePCM kind kjoin.
+Parameter kind_sep: @Sep_alg kind kjoin.
+Parameter kind_cross: @Cross_alg kind kjoin.
+Existing Instance kind_ppcm.
+Existing Instance kind_sep.
+
 (* Validity of traces.  The "valid" predicate ensures that related addresses don't get
     split apart from each other.  *)
-Parameter kind: Type.
 Parameter valid : (address -> option (pshare * kind)) -> Prop.
 Parameter valid_empty: valid (fun _ => None).
 Parameter valid_join: forall f g h : address -> option (pshare * kind),
@@ -20,16 +28,32 @@ End ADR_VAL.
 Module Type ADR_VAL0.
 Parameter address : Type.
 Parameter some_address:address.
+(* Kinds form a separation algebra *)
 Parameter kind: Type.
+Parameter kjoin: Join kind.
+(*Parameter kind_pcm: @PCM kind kjoin.*)
+Parameter kind_ppcm: @PrePCM kind kjoin.
+Parameter kind_sep: @Sep_alg kind kjoin.
+Parameter kind_cross: @Cross_alg kind kjoin.
+Existing Instance kind_ppcm.
+Existing Instance kind_sep.
 End ADR_VAL0.
 
 Module SimpleAdrVal (AV0: ADR_VAL0) <: 
    ADR_VAL with Definition address := AV0.address
-                   with Definition kind := AV0.kind.
+    with Definition kind := AV0.kind
+    with Definition kjoin := AV0.kjoin
+    with Definition kind_sep := AV0.kind_sep
+    with Definition kind_ppcm := AV0.kind_ppcm
+    with Definition kind_cross := AV0.kind_cross.
   Import AV0.
   Definition address := address.
   Definition some_address := some_address.
   Definition kind := kind.
+  Definition kind_sep := kind_sep.
+  Definition kind_ppcm := kind_ppcm.
+  Definition kind_cross := kind_cross.
+  Definition kjoin := kjoin.
   Definition valid (_: address -> option (pshare * kind)) := True.
   Lemma valid_empty: valid (fun _ => None).
   Proof. unfold valid; auto. Qed.
@@ -159,9 +183,10 @@ Module StratModel (AV' : ADR_VAL) : STRAT_MODEL with Module AV:=AV'.
     | res_join_NO1 : res_join PRED (NO' PRED) (NO' PRED) (NO' PRED)
     | res_join_NO2 : forall sh k p, res_join PRED (NO' PRED) (YES' PRED sh k p) (YES' PRED sh k p)
     | res_join_NO3 : forall sh k p, res_join PRED (YES' PRED sh k p) (NO' PRED) (YES' PRED sh k p)
-    | res_join_YES : forall (sh1 sh2 sh3:pshare) k p,
+    | res_join_YES : forall (sh1 sh2 sh3:pshare)(k1 k2 k3:kind) p,
       join sh1 sh2 sh3 ->
-      res_join PRED (YES' PRED sh1 k p) (YES' PRED sh2 k p) (YES' PRED sh3 k p)
+      kjoin k1 k2 k3 ->
+      res_join PRED (YES' PRED sh1 k1 p) (YES' PRED sh2 k2 p) (YES' PRED sh3 k3 p)
     | res_join_PURE : forall k p, res_join PRED (PURE' PRED k p) (PURE' PRED k p) (PURE' PRED k p).
 
  Instance Join_res (PRED: Type) : Join (res PRED) := res_join PRED.
@@ -171,8 +196,10 @@ Module StratModel (AV' : ADR_VAL) : STRAT_MODEL with Module AV:=AV'.
 
       (* saf_eq *)
       intros x y z z' H1 H2; inv H1; inv H2; auto.
-      f_equal. eapply join_eq; eauto.
-  
+      f_equal.
+      eapply join_eq; eauto.
+      eapply join_eq; eauto.
+      
       (* saf_assoc *)
       intros a b c d e H1 H2.
       icase d. exists c. inv H1. inv H2; split; constructor.
@@ -181,15 +208,30 @@ Module StratModel (AV' : ADR_VAL) : STRAT_MODEL with Module AV:=AV'.
       icase a. 3: elimtype False; inv H1. exists e. inv H1. split; auto. icase e. constructor. constructor. inv H2.
       icase e. 3: elimtype False; inv H2. elimtype False. inv H2.
       destruct (@join_assoc _ _ _ p5 p3 p1 p p7) as [sh' [? ?]]. inv H1; auto. inv H2; auto.
-      exists (YES' PRED sh' k p0).
+      destruct (@join_assoc _ _ _ k2 k1 k0 k k3) as [k' [? ?]]. inv H1; auto. inv H2; auto.
+      exists (YES' PRED sh' k' p0).
       inv H1. inv H2. split; constructor; auto.
       exists (PURE' PRED k p). inv H1. inv H2. split; constructor.
 
       (* saf_com *)
       intros a b c H; inv H; econstructor.
       apply join_comm; auto.
+      apply join_comm; auto.
 
-     intros; inv H; inv H0; auto. f_equal. eapply join_positivity; eauto.
+      (* saf_positivity *)
+      intros; inv H; inv H0; auto.
+      replace sh3 with sh1 in * by (eapply join_positivity; eauto).
+        eapply join_comm in H1; eapply join_comm in H6.
+        generalize (pshare_not_identity sh2); intros contra.
+        contradict contra.
+        Lemma join_unp : forall a b c,
+                           @join pshare _ a b c ->
+                           @join share _ a b c.
+          intros. inv H. constructor; unfold lifted_obj in *; auto.
+        Qed.
+        apply join_unp in H1. (*It has some effect but you can't see it! *)
+        eapply unit_identity in H1; assumption.
+
  Qed.
 
   Instance sa_rj : forall PRED, @Sep_alg _ (res_join PRED).
@@ -199,12 +241,12 @@ Module StratModel (AV' : ADR_VAL) : STRAT_MODEL with Module AV:=AV'.
             intros. inversion H; auto.
   Defined.
 
-  Instance ca_rj : forall PRED, @Canc_alg _ (res_join PRED).
+  (*Instance ca_rj : forall PRED, @Canc_alg _ (res_join PRED).
   Proof. repeat intro. inv H; inv H0; auto.
-    apply no_units in H2; contradiction.
+    apply no_units in H3; contradiction.
     apply no_units in H1; contradiction.
     f_equal; auto. eapply join_canc; eauto.
-  Qed.
+  Qed.*)
 
   Instance da_rj : forall PRED, @Disj_alg _ (res_join PRED).
   Proof.  repeat intro.
